sample_mark/verif_dispose.v
@@ -33,7 +33,7 @@ Definition spanning_spec :=
   DECLARE _spanning
   WITH sh: share, g: Graph, x: pointer_val
   PRE [ _x OF (tptr (Tstruct _Node noattr))]
-          PROP  (writable_share sh; vvalid (pg_gg g) x)
+          PROP  (writable_share sh; vvalid (pg_gg g) x; unmarked g x)
           LOCAL (temp _x (pointer_val_val x))
           SEP   (`(graph sh x g))
   POST [ Tvoid ]
@@ -63,9 +63,116 @@ Definition Vprog : varspecs := nil.
 
 Definition Gprog : funspecs := mark_spec :: spanning_spec :: dispose_spec :: main_spec::nil.
 
-Lemma body_mark: semax_body Vprog Gprog f_spanning spanning_spec.
+Lemma body_spanning: semax_body Vprog Gprog f_spanning spanning_spec.
 Proof.
   start_function.
-  assert (isptr (pointer_val_val x)). admit.
-  forward l_old.
+  remember (vgamma g x) as dlr eqn:?H.
+  destruct dlr as [[d l] r].
+  assert (d = false). {
+    hnf in H1. simpl in H1. unfold Ensembles.In in H1.
+    simpl in H2. unfold gamma in H2. destruct (vlabel g x) eqn:? .
+    symmetry in Heqb. specialize (H1 Heqb). exfalso; auto.
+    inversion H2. auto.
+  } subst.
+
+  localize
+   (PROP  ()
+    LOCAL (temp _x (pointer_val_val x))
+    SEP   (`(data_at sh node_type (Vint (Int.repr 0), (pointer_val_val l, pointer_val_val r))
+                     (pointer_val_val x)))).
+  
+  (* begin l = x -> l; *)
+  apply -> ram_seq_assoc.
+  eapply semax_ram_seq;
+    [ repeat apply eexists_add_stats_cons; constructor
+    | new_load_tac 
+    | abbreviate_semax_ram].
+  apply ram_extract_exists_pre.
+  intro l_old; autorewrite with subst; clear l_old.
+  (* end l = x -> l; *)
+
+  (* begin r = x -> r; *)
+  apply -> ram_seq_assoc.
+  eapply semax_ram_seq;
+    [ repeat apply eexists_add_stats_cons; constructor
+    | new_load_tac 
+    | abbreviate_semax_ram].
+  apply ram_extract_exists_pre.
+  intro r_old; autorewrite with subst; clear r_old.
+  (* end r = x -> r; *)
+
+  (* begin x -> m = 1; *)
+  apply -> ram_seq_assoc.
+  eapply semax_ram_seq;
+    [ repeat apply eexists_add_stats_cons; constructor
+    | new_store_tac
+    | abbreviate_semax_ram].
+  cbv beta zeta iota delta [replace_nth].
+  change (@field_at CompSpecs CS_legal sh node_type []
+           (Vint (Int.repr 1), (pointer_val_val l, pointer_val_val r))) with
+         (@data_at CompSpecs CS_legal sh node_type
+                   (Vint (Int.repr 1), (pointer_val_val l, pointer_val_val r))).
+  (* end x -> m = 1; *)
+  
+  unlocalize (PROP ()
+              LOCAL  (temp _r (pointer_val_val r); temp _l (pointer_val_val l); temp _x (pointer_val_val x))
+              SEP  (`(graph sh x (Graph_gen g x true)))).
+  Grab Existential Variables.
+  Focus 6. { solve_split_by_closed. } Unfocus.
+  Focus 2. { entailer!. } Unfocus.
+  Focus 3. { entailer!. } Unfocus.
+  Focus 3. { repeat constructor; auto with closed. } Unfocus.
+  Focus 2. {
+    entailer!.
+    rewrite Graph_gen_spatial_spec by eauto.
+    pose proof (@graph_ramify_aux0 _ _ _ _ _ _ _ (SGA_VST sh) g _ x (false, l, r) (true, l, r)).
+    simpl in H4; auto.
+  } Unfocus.
+
+  (* if (l) { *)
+  apply -> ram_seq_assoc.
+  symmetry in H2.
+  pose proof Graph_gen_true_mark1 g x _ _ H2 H0.
+  assert (H_GAMMA_g1: vgamma (Graph_gen g x true) x = (true, l, r)) by
+   (rewrite (proj1 (proj2 (Graph_gen_spatial_spec g x _ true _ _ H2))) by assumption;
+    apply spacialgraph_gen_vgamma).
+  forget (Graph_gen g x true) as g1.
+  unfold semax_ram.
+  forward_if_tac
+    (PROP  ()
+     LOCAL (temp _r (pointer_val_val r);
+            temp _l (pointer_val_val l);
+            temp _x (pointer_val_val x))
+     SEP (`(EX g2: Graph, !! spanning_tree g1 l g2 && graph sh x g2))).
+
+  (* root_mark = l -> m; *)
+  localize
+    (PROP  ()
+     LOCAL  (temp _l (pointer_val_val l))
+     SEP  (`(data_at sh node_type (vgamma2cdata (vgamma g1 l)) (pointer_val_val l)))).
+  remember (vgamma g1 l) as dlr in |-*.
+  destruct dlr as [[dd ll] rr].
+  eapply semax_ram_seq;
+    [ repeat apply eexists_add_stats_cons; constructor
+    | new_load_tac 
+    | abbreviate_semax_ram].
+  apply ram_extract_exists_pre.
+  intro root_mark_old; autorewrite with subst; clear root_mark_old.
+  replace (if dd then 1 else 0) with (if node_pred_dec (marked g1) l then 1 else 0).
+  Focus 2. {
+    destruct (node_pred_dec (marked g1)); destruct dd; auto; symmetry in Heqdlr.
+    apply vgamma_is_false in Heqdlr. simpl in a. unfold unmarked in Heqdlr. hnf in Heqdlr.
+    unfold Ensembles.In in Heqdlr. simpl in Heqdlr. apply Heqdlr in a. exfalso; auto.
+    apply vgamma_is_true in Heqdlr. exfalso; auto.
+  } Unfocus.
+  rewrite Heqdlr.
+  unlocalize
+    (PROP  ()
+     LOCAL (temp _root_mark (Vint (Int.repr (if node_pred_dec (marked g1) l then 1 else 0)));
+            temp _r (pointer_val_val r);
+            temp _l (pointer_val_val l);
+            temp _x (pointer_val_val x))
+     SEP  (`(graph sh x g1))).
+  
+  (* assert (isptr (pointer_val_val x)). admit. *)
 Abort.
