sample_mark/env_dispose.v
@@ -3,6 +3,7 @@ Require Export RamifyCoq.floyd_ext.semax_ram_lemmas.
 Require Export RamifyCoq.floyd_ext.exists_trick.
 Require Export RamifyCoq.floyd_ext.closed_lemmas.
 Require Export RamifyCoq.floyd_ext.comparable.
+Require Export RamifyCoq.floyd_ext.semax_ram_tac.
 Require Export RamifyCoq.sample_mark.dispose.
 
 Local Open Scope logic.
